theories/Util.v
@@ -1,0 +1,31 @@
+From Coq Require Import Utf8 List.
+From Equations Require Import Equations.
+
+Import ListNotations.
+
+Set Default Goal Selector "!".
+
+Ltac forall_iff_impl T :=
+  lazymatch eval cbn beta in T with
+  | forall x : ?A, @?T' x =>
+    let y := fresh x in
+    refine (forall y, _) ;
+    forall_iff_impl (@T' x)
+  | ?P ↔ ?Q => exact (P → Q)
+  | _ => fail "not a quantified ↔"
+  end.
+
+Ltac wlog_iff_using tac :=
+  lazymatch goal with
+  | |- ?G =>
+    let G' := fresh in
+    unshelve refine (let G' : Prop := _ in _) ; [ forall_iff_impl G |] ;
+    let h := fresh in
+    assert (h : G') ; [
+      subst G'
+    | subst G' ; intros ; split ; eauto ; apply h ; clear h ; tac
+    ]
+  end.
+
+Ltac wlog_iff :=
+  wlog_iff_using firstorder.
